VerseRocq/verse/densem/PFun.v
@@ -7,9 +7,11 @@ Require Import structures.List.
 
 Import ListNotations.
 
-Definition PFun A B := list (A * B)%type.
+Definition pfun A B := list (A * B)%type.
 
-Definition dom {A B} : PFun A B -> list A := map fst.
+Module PFun.
+
+Definition dom {A B} : pfun A B -> list A := map fst.
 
 Section PFun.
 
@@ -20,7 +22,7 @@ Definition A_eq : A -> A -> Prop :=
 
 Context `{EQA : Equivalence A A_eq}.
 
-Fixpoint apply_opt (f : PFun A B) (x : A) : option B := 
+Fixpoint apply_opt (f : pfun A B) (x : A) : option B := 
   match f with 
     | [] => None
     | (y,b) :: xs => 
@@ -50,7 +52,7 @@ Section Eqb.
 
 Variable B_eqb : B -> B -> bool.
 
-Definition eqb : PFun A B -> PFun A B -> bool := 
+Definition eqb : pfun A B -> pfun A B -> bool := 
   List.forallb2 (fun '(x1,y1) '(x2, y2) => (A_eqb x1 x2 && B_eqb y1 y2)%bool).
 
 End Eqb.
@@ -61,7 +63,7 @@ Variable A_compare : A -> A -> comparison.
 Variable B_compare : B -> B -> comparison.
 
 Definition compare   
-  (xs: PFun A B) (ys: PFun A B) : comparison := 
+  (xs: pfun A B) (ys: pfun A B) : comparison := 
   list_compare (fun '(x1,y1) '(x2, y2) => 
                   match A_compare x1 x2 with 
                   | Lt => Lt
@@ -74,14 +76,24 @@ Definition A_lt : A -> A -> Prop :=
 Definition A_ltb x y := 
   match A_compare x y with | Lt => true | _ => false end.
 
-Section Valid.
 
-Context `{SOA : StrictOrder A A_lt}.
-
-Definition valid : PFun A B -> Prop := fun f => LocallySorted A_lt (dom f).
+(* intersection of two partial maps *)
+Fixpoint intersect (l1 l2 : pfun A B) := 
+  let fix aux l2 :=
+  match l1, l2 with
+  | [], _ => []
+  | _, [] => []
+  | (a1,b1)::l1', (a2,b2)::l2' =>
+      match A_compare a1 a2 with 
+      | Lt =>  intersect l1' l2
+      | Eq =>  (a2,b2) :: intersect l1' l2'
+      | Gt =>  aux l2'
+      end
+  end
+  in aux l2.
 
 (* right-biased union of two partial maps. *)
-Fixpoint merge (l1 l2 : PFun A B) :=
+Fixpoint merge (l1 l2 : pfun A B) :=
   let fix merge_aux l2 :=
   match l1, l2 with
   | [], _ => l2
@@ -95,6 +107,18 @@ Fixpoint merge (l1 l2 : PFun A B) :=
   end
   in merge_aux l2.
 
+
+Section Valid.
+
+Context `{SOA : StrictOrder A A_lt}.
+
+Definition valid : pfun A B -> Prop := fun f => LocallySorted A_lt (dom f).
+
+
+Lemma intersect_valid {f g} : valid f -> valid g -> valid (intersect f g).
+Proof. 
+Admitted.
+  
 Lemma merge_valid : forall f g, valid f -> valid g -> valid (merge f g).
 Proof. induction f.
        - intros. unfold merge. destruct g. auto. auto.
@@ -108,5 +132,14 @@ Admitted.
 End Valid.
 End Compare.
 End PFun.     
+End PFun.
 
 
+Declare Scope pfun_scope.
+Delimit Scope pfun_scope with pfun.
+
+Module PFunNotation.
+Notation "∅" := nil : pfun_scope.
+Infix "∩" := PFun.intersect (at level 90) : pfun_scope.
+Infix "∪" := PFun.merge (at level 90) : pfun_scope.
+End PFunNotation.
